

0.1 Mixed Foundations Review

[← Contents](#)[✓ Solutions](#)

Mixed Foundations Review

Chapter 0 — Absolute Foundations

Show all work. Use PEMDAS. Rewrite subtraction as “add the opposite.” Distribute to every term. Keep track of negative signs carefully.

Name: _____ Date: _____

Skills This Review Mixes

- **Integers & signs:** adding/subtracting negatives; multiplying/dividing signs; rewriting subtraction.
- **Distributive property:** $a(b + c) = ab + ac$ and $-(b - c) = -b + c$.
- **Order of operations:** parentheses, exponents, multiply/divide left to right, add/subtract left to right.
- **Simplify & solve:** combine like terms, then isolate the variable.

Part A — Evaluate & Simplify (Warm-Up)

Evaluate or simplify.

1. $8 - 3 \cdot (5 - 7)$

2. $-12 + 4 \cdot 3 - 6$

3. $24 \div 3 \cdot 2 - 5$

4. $-(6 - 14) + 2^3$

5. $-3(2 - (5 - 9))$

6. $5 - (3 - (2 - 7))$

7. $-2^3 + 10$

8. $(-2)^3 + 10$

Part B — Distribute, Then Combine Like Terms

Simplify completely.

1. $-(x + 7) + 3x$

2. $2(3x - 5) - (x - 4)$

3. $-(4x - 9) - 2(x + 3)$

4. $5 - 3(2x - 1)$

5. $-2(3y - 8) + (y - 5)$

6. $4(2a - (a - 6))$

7. $-(2m - 3n + 4) + 2(m + n)$

Part C — Solve Equations (Watch the Signs)

Solve for the variable. Check by substitution when you can.

1. $x - 9 = -4$

2. $-7 = x + 3$

3. $-3x = 24$

4. $\frac{x}{-6} = -5$

5. $2x - 5 = 11$

6. $-4x + 9 = -19$

7. $3(x - 4) = -18$

8. $-2(x + 7) = 10$

9. $5 - (x - 3) = -4$

10. $2(3x - 1) - 4 = 8$

Part D — Multi-Step (All Skills Together)

Simplify first, then solve.

1. $3 - (2x - 7) = 10$

2. $-(4x - 5) + 2x = 13$

3. $2(x - 6) - 3(x + 1) = -8$

4. $5(2x - 3) + 4 = 3(3x + 2)$

5. $\frac{1}{2}(6x - 8) - (x - 3) = 5$

Challenge (optional)

These are harder. Take your time and write neat steps.

1. A student earns \$12 per hour. They worked 5 hours, but had a \$8 fee taken out. Write and evaluate an expression for their pay.
2. The temperature was -3°F . Overnight it dropped 7 degrees, then rose 5 degrees. What is the final temperature?

3. Solve and interpret: $-2(x - 4) + 3 = 17$. (What number makes the equation true?)

4. True or false? Explain: $-(a - b) = -a - b$.